#+TITLE: Chapter 5: Binomial Coefficients

* Basic Identities

** Binomial Coefficient Definition

${r \choose k} = \frac{r(r-1)...(r - k + 1)}{k(k - 1)...(1)} = \frac{r^{\underline{k}}}{k!}$ if $k \geq 0$, $0$ otherwise

This definition has several noteworthy features:

1. The letter $r$ emphasizes the fact that binomial coefficients make sense when any real number appears in this position
2. We can view $(\frac{r}{k})$ as a kth degree polynomial in r
3. We haven't defined binomial coefficients for noninteger lower indices.

** Binomial Coefficient with Factorials

 ${n \choose k} = \frac{n!}{k!(n - k)!}$ where $n \geq k \geq 0$

** Symmetry Identity

${n \choose k} = {n \choose n - k}$

for integers $n, k, n \geq 0$

** Absorption Identity

${r \choose k} = \frac{r}{k}{r - 1 \choose k - 1}$ where $k \neq 0$

Alternatively, we can use the following that works even when $k = 0$

$k{r \choose k} = r{r - 1 \choose k - 1}$

We can even do one where we keep the lower index intact

$(r - k){r \choose k} = r{r - 1 \choose k}$

** Addition Formula

${r \choose k} = {r - 1 \choose k} + {r - 1 \choose k - 1}$ where $k \in \mathcal{Z}$

** Expansion from the Highest Index (parallel summation identity)

$\Sigma_{k \leq n} {r + k \choose k} = {r \choose 0} + {r + 1 \choose 1} + ... + {r + n \choose n} = {r + n + 1 \choose n}$

** Expansion from the Lowest Index

$\Sigma_{k \leq n} {k \choose m} = {0 \choose m} + {1 \choose m} + ... + {n \choose m} = {n + 1 \choose m + 1}$

** Indefinite Summation Formula

$\Sigma {x \choose m} \delta x = {x \choose m + 1} + C$

** Binomial Theorem

$(x + y)^r = \Sigma_k {r \choose k} x^ky^{r - k}$ where $r \in \mathcal{Z}, r \geq 0$ or $|x/y| < 1$

** Binomial Theorem for Special Case $y = 1$ and $r$ is not a non-negative integer

$(1 + z)^r = \Sigma_k {r \choose k} z^k$ where $|z| < 1$

** Pascal's Triangle for Negative $n$

${r \choose k} = (-1)^k{k - r - 1 \choose k}$

The transformation above is called /negating the upper index/

** Moving Quantities between Upper and Lower Index Positions

$(-1)^m{-n -1 \choose m} = (-1)^n{-m - 1 \choose n}$

** Partial Sum of the rth row of Pascal's Triangle, if the row has been given alternating signs

$\Sigma_{k \leq m} {r \choose k}(-1)^k = (-1)^m{r - 1 \choose m}$

** Partial Sum of the Row Elements if they have been multiplied by their distance from the center

$\Sigma_{k \leq m}{r \choose k}(\frac{r}{2} - k) = \frac{m + 1}{2}{r \choose m + 1}$

** Identity

$\Sigma_{k \leq m}{m + r \choose k}x^ky^{m - k} = \Sigma_{k \leq m}{-r \choose k}(-x)^k(x + y)^{m - k}$

** Combinatorial Formula for $2^m$

$\Sigma_{k \leq m}{m + k \choose k}2^{-k} = 2^m$

** Rule for Simplifying the Product of 2 Binomial Coefficients

${r \choose m}{m \choose k} = {r \choose k}{r - k \choose m - k}$

The special case for $k = 1$ is the absorption identity

The LHS uses $m$ twice, whereas the RHS uses $m$ once. This is a handy transformation to use before summing on $m$

** Trinomial Coefficient

${a + b + c \choose a, b, c} = \frac{(a + b + c)!}{a!b!c!}$

** Trinomial Theorem

$(x + y + z)^n = \Sigma_{0 \leq a,b,c \leq n, a + b + c = n} \frac{(a + b + c)!}{a!b!c!}x^ay^bz^c = \Sigma_{0 \leq a,b,c \leq n, a + b + c = n} {a + b + c \choose b + c}{b + c \choose c} x^ay^bz^c$

** Multinomial Coefficients

${a_1 + a_2 + ... + a_m \choose a_1, a_2, ..., a_m} = \frac{(a_1 + a_2 + ... + a_m)!}{a_1!a_2!...a_m!} = {a_1 + a_2 + ... + a_m \choose a_2 + ... + a_m} ... {a_{m - 1} + a_m \choose a_m}$

** Vandermonde's Convolution

$\Sigma_k {r \choose m + k}{s \choose n - k} = {r + s \choose m + n}$

There are some other hairier identities for sums on trinomial and multinomial coefficients that I didn't write down

* Basic Practice

On problem 7

** Identity for Division of Same Indexed Binomial Coefficients

$\Sigma_{j = 0}^m {m \choose j} {r \choose j}^{-1} = \frac{r + 1}{r + 1 - m}$

where $m \in \mathcal{Z}^{+}$ and $r \notin \{0, 1, ..., m - 1\}$

* Tricks of the Trade

** Trick 1: Going Halves

*** Duplication Formula (5.34)

$r^{\underline{k}}(r - \frac{1}{2})^{\underline{k}} = (2r)^{\underline{2k}}/2^{2k}$

*** Duplication Identity (5.35)

${r \choose k} {r - 1/2 \choose k} = {2r \choose 2k} {2k \choose k} / 2^{2k}$

*** Duplication Identity with k = r = n (5.36)

${n - 1/2 \choose n} = {2n \choose n} / 2^{2n}$

*** Duplication Identity with Negation of Upper Index (5.37)

${-1/2 \choose n} = (\frac{-1}{4})^n {2n \choose n}$

*** Corollary to (5.35)

$\Sigma_k {n \choose 2k} {2k \choose k} 2^{-2k} = {n - 1/2 \choose \left\lfloor{n/2}\right\rfloor}$

*** Property of the Middle Elements of Pascal's Triangle

$\Sigma_k {2k \choose k} {2n - 2k \choose n - k} = 4^n$

** Trick 2: High-Order Differences

*** High-Order Difference Operation (5.40)

$\Delta^n f(x) = \Sigma_k {n \choose k} (-1)^{n - k}f(x + k)$

*** Partial Fraction Expansion of $n! / (x (x + 1) ... (x + n))$ (5.41)

$\Sigma_k {n \choose k} \frac{(-1)^k}{x + k} = x^{-1} {x + n \choose n}^{-1}$

*** Newton Series

Any polynomical can be represented as a sum of multiples of binomial coefficients

$f(x) = c_d {x \choose d} + c_{d - 1} {x \choose d - 1} + ... + c_1 {x \choose 1} + c_0 {x \choose 0}$

where $c_k = k!b_k$ for $0 \leq k \leq d$

The nth difference of a Newton series is

$\Delta^n f(x) = c_d {x \choose d - n} + c_{d - 1} {n \choose d - 1 - n} + ... + c_1 {x \choose 1 - n} + c_0 {x \choose - n}$

*** Alternating polynomial sum (5.42)

$\Sigma_k {n \choose k} (-1)^k (a_0 + a_1 k + ... + a_n k^n) = (-1)^n n! a_n$

*** Sum Identity (5.43)

$\Sigma_k {n \choose k} {r - sk \choose n} (-1)^k = s^n$

*** $\Delta^n f(0) = c_n$ in the infinite case (5.44)

$f(x) = f(0){x \choose 0} + \Delta f(0) {x \choose 1} + \Delta^2 f(0) {x \choose 2} + \Delta^3 f(0) {x \choose 3}$ + ...

*** Newton Series Analogue to Taylor Series (5.45)

$g(a + x) = \frac{g(a)}{0!}x^{\underline{0}} + \frac{\Delta g(a)}{1!}x^{\underline{1}} + \frac{\Delta^2 g(a)}{2!}x^{\underline{2}}$ + ...

** Trick 3: Inversion

*** Inversion Formula (5.48)

$g(n) = \Sigma_k {n \choose k}(-1)^kf(k) \iff f(n) = \Sigma_k {n \choose k}(-1)^kg(k)$

The dual relationship between $f$ and $g$ is called an inversion formula

*** Subfactorial formulation of factorial (5.49)

$n! = \Sigma_k h(n, k) = \Sigma_k {n \choose k}(n - k)_i = \Sigma_k {n \choose k} k_i$

where i is the subfactorial function

*** Subfactorial Summation Almost Closed Form (5.50)

$n_i = n! \Sigma_{0 \leq k \leq n} \frac{(-1)^k}{k!}$

*** Subfactorial Summation Closed Form (5.51)

$n_i = \left\lfloor{\frac{n!}{e} + \frac{1}{2}}\right\rfloor + [n = 0]$

* 5.4 | Generating Functions
** Power Series (5.52)

An infinite sequence $<a_0, a_1, a_2, ...>$ that we wish to deal with in some way can conveniently be represented as a power series in an auxiliary variable z,

$A(z) = a_0 + a_1z + a_2z^2 + ... = \Sigma_{k \geq 0} a_k z^k$

** Notation: Coefficient of a Power Series (5.53)

$[z^n]A(z) = a_n$

or, in other words $[z^n]A(z)$ is the coefficient of $z^n$ in $A(z)$

** Convolution of Sequences (5.54)

If we wish to evaluate any sum that has the general form

$c_n = \Sigma_{k = 0}^n a_k b_{n - k}$

and if we know the generating functions $A(z), B(z)$ we have

$c_n = [z^n]A(z)B(z)$

The sequence $<c_n>$ defined by above is called the convolution of the sequences $<a_n>, <b_n>$; two sequences are convolved by forming the sums of all products whose subscripts add up to a given amount.

The gist is that convolution of sequences corresponds to multiplication of their generating functions

** Another Convolution Identity (5.55)

$\Sigma_{k = 0}^n {r \choose k} {r \choose n - k}(-1)^k = (-1)^{n/2}{r \choose n/2}[n \mathrm{even}]$

** Fixed Lower Index Varying Upper Index Identities (5.56, 5.57)

$\frac{1}{(1 - z)^{n + 1}} = \Sigma_{k \geq 0} {n + k \choose n}z^k$

$\frac{z^n}{(1 - z)^{n + 1}} = \Sigma_{k \geq 0} {k \choose n}z^k$

** Generalized Binomial Series & Generalized Exponential Series (5.58)

$\mathcal{B}_t(z) = \Sigma_{x \geq 0} (tk)^{\underline{k - 1}}\frac{z^k}{k!}$

$\mathcal{E}_t(z) = \Sigma_{k \geq 0} (tk + 1)^{k - 1} \frac{z^k}{k!}$

** Identities of Generalized Binomial/Exponential Series (5.59 - 5.65)

$\mathcal{B}_t(z)^{1 - t} - \mathcal{B}_t(z)^{-t} = z$

$\mathcal{E}_t(z)^{-t} \ln \mathcal{E}_t(z) = z$


#+DOWNLOADED: screenshot @ 2021-11-19 09:05:38
[[file:5.4_|_Generating_Functions/2021-11-19_09-05-38_screenshot.png]]


#+DOWNLOADED: screenshot @ 2021-11-19 09:05:46
[[file:5.4_|_Generating_Functions/2021-11-19_09-05-46_screenshot.png]]

** $\mathcal{E}_1$ (5.66)

$\mathcal{E}(z) = \Sigma_{k \geq 0} z^k = \frac{1}{1 - z}$

** Generalized Exponential Series Identity (5.67)

$\mathcal{E}(z) = e^{z \mathcal{E}(z)}$

** Generalized Binomial with t = 2, t = -1 (5.68 - 5.73)


#+DOWNLOADED: screenshot @ 2021-11-19 09:10:33
[[file:5.4_|_Generating_Functions/2021-11-19_09-10-33_screenshot.png]]

** Catalan Numbers

The coefficients ${2n \choose n}\frac{1}{n+1}$ of $\mathcal{B}_2(z)$ are called Catalan numbers $C_n$

where the sequence begins as follows:

$C_n = 1, 1, 2, 5, 14, 42, 132, 429, 1430, 4862, 16796$, ...

* Hypergeometric Functions

It's natural to ask if there is a unifying principle that will systematically handle a great variety of binomial coefficient summations all at once. The answer is yes, and it is based on the theory of certain infinite sums called *hypergeometric series*

** Hypergeometric Series (5.76)

The hypergeometric series is a power series in $z$ with $m + n$ parameters. Below is an attempted latex representation with rising factorial powers:

$F({a_1, ..., a_m \choose b_1, ..., b_m}|z) = \Sigma_{k \geq 0} \frac{a_1^{\overline{k}} ... a_m^{\overline{k}}}{b_1^{\overline{k}} ... b_m^{\overline{k}}} \frac{z^k}{k!}$

To avoid division by 0, none of the b's may be 0 or a negative integer

The notation

$F(a_1,..., a_m;b_1, ..., b_m; z)$ is also used as an alternative

The a's are called upper arguments, the b's are called lower arguments, the z is called the argument

** Closed Form for m = 1, n = 0 (5.77)

$F(a, 1; 1; z) = \frac{1}{(1 - z)^a}$

** Modified Bessel Function of order b - 1 (5.78)

$F(1; b, 1; z) = \Sigma_{k \geq 0} \frac{(b - 1)!}{(b - 1 + k)!} \frac{z^k}{k!}  = I_{b - 1}(z \sqrt(z)) \frac{(b - 1)!}{z^{(b - 1)/2}}$

** Confluent Hypergeometric Series (m = n = 1) (5.79)

$F(a;b;z) = \Sigma_{k \geq 0}\frac{a^{\overline{k}}}{b^{\overline{k}}}\frac{z^k}{k!} = M(a, b, z)$

** Gaussian Hypergeometric Series (5.80)

$F(a,b;c;z) = \Sigma_{k \geq 0}\frac{a^{\overline{k}}b^{\overline{k}}z^k}{c^{\overline{k}}k!}$

** Rational Function of k (5.81)

$\frac{t_{k + 1}}{t_{k}} = \frac{(k + a_1)...(k + a_m)z}{(k + b_1)...(k + b_n)(k + 1)}$

This is the rational function of k, that is, a quotient of polynomials in k.
The hypergeometric series are precisely those series whose first term is 1 and whose term ratio t-k+1/t-k is a rational function of k

This allows us to write a representation of the hypergeometric representation of a given quantity when it is possible.

** Factorial Function defined for all complex numbers (5.83)

$\frac{1}{z!} = \lim_{n \to \infty} {n+z \choose n} n^{-z}$

** Integral Definition of the Factorial Function (5.84)

$z! = \int_0^{\infty} t^ze^{-t} dt$ if $\mathcal{R}(z) > - 1$

** Gamma Function Formulation of Factorial (5.86, 5.87)

$\Gamma(z + 1) = z!$

$(-z)!\Gamma{(z)} = \frac{\pi}{\sin \pi z}$

** Generalized Factorial Powers where $z, w \in \mathcal{C}$ (5.88, 5.89, 5.90)

$z^{\underline{w}} = \frac{z!}{(z - w)!}$

$z^{\overline{w}} = \frac{\Gamma(z + w)}{\Gamma(z)}$

${z \choose w} = \lim_{\xi \to z} \lim_{\omega \to w} \frac{\xi!}{\omega!(\xi - \omega)!}$ where $z, w \in \mathcal{C}$

** Vandermonde's Convolution in Hypergeometric Form (5.92)

$F(a, b; c; 1) = \frac{\Gamma(c - a - b) \Gamma(c)}{\Gamma(c - a) \Gamma(c - b)}$

when integer $b > 0$ or $\mathcal{R}c > \mathcal{R}a + \mathcal{R}b$
otherwise the series doesn't converge

** Kummer's Formula (5.94)

$F(a, b; 1 + b - a; -1) = \frac{(b/2)!}{b!} (b - a)^{\underline{b/2}}$

* Hypergeometric Transformations

** Pfaff's Reflection Law (5.101)

$\frac{1}{(1 - z)^a} F(a, b; c; \frac{-z}{1 - z}) = F(a, c-b; c; z)$

Skimmed a bunch about using hypergeometric transformations for differential equations

* Partial Hypergeometric Sums

most notably, Gosper's algorithm:

Gosper's algorithm is a procedure for finding sums of hypergeometric terms that are themselves hypergeometric terms.
That is: suppose one has $a(1) + ... + a(n) = S(n) − S(0)$, where $S(n)$ is a hypergeometric term (i.e., $S(n + 1)/S(n)$ is a rational function of n); then necessarily $a(n)$ is itself a hypergeometric term, and given the formula for $a(n)$ Gosper's algorithm finds that for $S(n)$.

Step 1: Find a polynomial p such that, writing $b(n) = a(n)/p(n)$, the ratio $b(n)/b(n − 1)$ has the form $q(n)/r(n)$ where q and r are polynomials and no $q(n)$ has a nontrivial factor with $r(n + j)$ for $j = 0, 1, 2$, ... . (This is always possible, whether or not the series is summable in closed form.)

Step 2: Find a polynomial ƒ such that $S(n) = q(n + 1)/p(n) f(n) a(n)$. If the series is summable in closed form then clearly a rational function ƒ with this property exists; in fact it must always be a polynomial, and an upper bound on its degree can be found. Determining ƒ (or finding that there is no such ƒ) is then a matter of solving a system of linear equations.

* Mechanical Summation

Gosper's algorithm finds a closed form for only a few of the binomial sums we meet in practice. Doron Zeilberger extended it, making it succeed in vastly more cases. This is called the Gosper-Zeilberger algorithm.


#+DOWNLOADED: screenshot @ 2021-12-05 21:14:59
[[file:Mechanical_Summation/2021-12-05_21-14-59_screenshot.png]]
