#+TITLE: Chapter 7: Generating Functions

* Domino Theory and Change

Fun! A sequence of nontrivial problems solved with generating functions and some nice looking TeX

* Basic Maneuvers

Our generic generating function has the form

$G(z) = g_0 + g_1z + g_2z^2 + ... = \Sigma_{n \geq 0} g_n z^n$

** Additioin of Generating Functions

$\alpha F(z) + \beta G(z) = \Sigma_n (\alpha f_n + \beta g_n)z^n$

** Shifting

To shift by m places to the *right*, simply muliply by z^m
This way we form a generating function for the sequence $<0, 0, ..., 0, g_0, g_1, ...>$

$z^m G(z) = \Sigma_n g_{n - m}z^n$

To shift by m places to the *left* we subtract off the first m terms and then divide by z^m

$\frac{1}{z^m} G(z) - (g_0 + g_1 z + ... + g_{m - 1}z^{m - 1}) = \Sigma_{n \geq 0} g_{n + m}z^n$

** Constant Multiple

$G(cz) = \Sigma_n g_n(cz)^n = \Sigma_n c^n g_n z^n$

** Differentiation to bring down a factor (7.17)

$G'(z) = \Sigma_n (n + 1) g_{n + 1}z^n$

which we can shift to the right

$z G'(z) = \Sigma_n n g_n z^n$

** Integration lets us divide by n (7.19)

$\int_0^z G(t) dt = \Sigma_{n \geq 1} \frac{1}{n} g_{n - 1} z^n$

** Multiplication / Convolution (7.20)

$F(z)G(z) = \Sigma_n ( \Sigma_k f_k g_{n - k})z^n$


#+DOWNLOADED: screenshot @ 2021-12-15 12:45:47
[[file:Basic_Maneuvers/2021-12-15_12-45-47_screenshot.png]]

* Solving Recurrences
